Move rename logic to own file.

IL/IL.v
@@ -123,35 +123,6 @@ Proof.
     eauto using notOccur, Exp.freeVars_disj_notOccur, list_union_notOccur'.
 Qed.
 
-
-Fixpoint rename (ϱ:env var) (s:stmt) : stmt :=
-  match s with
-    | stmtLet x e s => stmtLet (ϱ x) (rename_exp ϱ e) (rename ϱ s)
-    | stmtIf e s t => stmtIf (rename_exp ϱ e) (rename ϱ s) (rename ϱ t)
-    | stmtApp l Y => stmtApp l (List.map (rename_exp ϱ) Y)
-    | stmtReturn e => stmtReturn (rename_exp ϱ e)
-    | stmtExtern x f e s => stmtExtern (ϱ x) f (List.map (rename_exp ϱ) e) (rename ϱ s)
-    | stmtFun Z s t => stmtFun (lookup_list ϱ Z) (rename ϱ s) (rename ϱ t)
-  end.
-
-(** Renaming respects function equivalence *)
-
-Global Instance rename_morphism
-  : Proper (@feq _ _ _eq ==> eq ==> eq) rename.
-Proof.
-  unfold Proper, respectful; intros; subst.
-  general induction y0; simpl; f_equal; eauto; try (now rewrite H; eauto);
-  eauto using rename_exp_ext, map_ext_get_eq; eauto.
-Qed.
-
-Lemma rename_agree ϱ ϱ' s
-: agree_on eq (occurVars s) ϱ ϱ'
-  -> rename ϱ s = rename ϱ' s.
-Proof with eauto 50 using rename_exp_agree, map_ext_get_eq with cset.
-  intros. general induction s; simpl in *; f_equal...
-Qed.
-
-
 Fixpoint label_closed (n:nat) (s:stmt) : Prop :=
   match s with
     | stmtLet _ _ s => label_closed n s
