Coherence/Allocation.v
@@ -2,7 +2,7 @@ Require Import CSet Le.
 
 Require Import Plus Util Map DecSolve.
 Require Import Env EnvTy IL Annotation Liveness Coherence Alpha Restrict RenamedApart.
-Require Import RenamedApart_Liveness.
+Require Import Rename RenamedApart_Liveness.
 
 Set Implicit Arguments.
 
