IL/Rename.v
@@ -1,0 +1,39 @@
+Require Import List.
+Require Export Util Relations Get Drop Var Val Exp Env Map CSet AutoIndTac MoreList OptionMap Events.
+Require Import SetOperations IL.
+
+Set Implicit Arguments.
+
+Fixpoint rename (ϱ:env var) (s:stmt) : stmt :=
+  match s with
+    | stmtLet x e s => stmtLet (ϱ x) (rename_exp ϱ e) (rename ϱ s)
+    | stmtIf e s t => stmtIf (rename_exp ϱ e) (rename ϱ s) (rename ϱ t)
+    | stmtApp l Y => stmtApp l (List.map (rename_exp ϱ) Y)
+    | stmtReturn e => stmtReturn (rename_exp ϱ e)
+    | stmtExtern x f e s => stmtExtern (ϱ x) f (List.map (rename_exp ϱ) e) (rename ϱ s)
+    | stmtFun Z s t => stmtFun (lookup_list ϱ Z) (rename ϱ s) (rename ϱ t)
+  end.
+
+(** Renaming respects function equivalence *)
+
+Global Instance rename_morphism
+  : Proper (@feq _ _ _eq ==> eq ==> eq) rename.
+Proof.
+  unfold Proper, respectful; intros; subst.
+  general induction y0; simpl; f_equal; eauto; try (now rewrite H; eauto);
+  eauto using rename_exp_ext, map_ext_get_eq; eauto.
+Qed.
+
+Lemma rename_agree ϱ ϱ' s
+: agree_on eq (occurVars s) ϱ ϱ'
+  -> rename ϱ s = rename ϱ' s.
+Proof with eauto 50 using rename_exp_agree, map_ext_get_eq with cset.
+  intros. general induction s; simpl in *; f_equal...
+Qed.
+
+
+(*
+*** Local Variables: ***
+*** coq-load-path: (("../" "Lvc")) ***
+*** End: ***
+*)
